common/Memory.v
@@ -176,6 +176,69 @@ Module Mem (P:Policy).
         * right; red; intros. elim n0. red; intros. apply H0; lia.
     - left; red; intros. extlia.
   Defined.
+
+  (** [valid_access m chunk ofs] holds if a memory access
+      of the given chunk is possible in [m] at address [ofs].
+      This means:
+      - The offset [ofs] is aligned.
+      - If any of the range of bytes accessed have permission [Dead],
+      they are not shadowed by the compiler
+   *)
+
+  Definition valid_access (m: mem) (chunk: memory_chunk) (ofs: Z): Prop :=
+    range_perm m ofs (ofs + size_chunk chunk) Live
+    /\ (align_chunk chunk | ofs).
+
+  Theorem valid_access_valid_addr:
+    forall m chunk ofs,
+      valid_access m chunk ofs ->
+      valid_addr m ofs.
+  Admitted.
+(*Proof.
+  intros. destruct H.
+  assert (perm m ofs Cur Nonempty).
+    apply H. generalize (size_chunk_pos chunk). lia.
+  eauto with mem.
+Qed. *)
+
+  Local Hint Resolve valid_access_valid_addr: mem.
+
+  Theorem valid_addr_valid_access:
+    forall m chunk ofs,
+      valid_addr m ofs ->
+      valid_access m chunk ofs.
+  Admitted.
+
+  Lemma valid_access_perm:
+    forall m chunk ofs,
+      valid_access m chunk ofs ->
+      perm m ofs Live.
+  Proof.
+    intros. destruct H. apply H. generalize (size_chunk_pos chunk). lia.
+  Qed.
+
+  Lemma valid_access_compat:
+    forall m chunk1 chunk2 ofs,
+      size_chunk chunk1 = size_chunk chunk2 ->
+      align_chunk chunk2 <= align_chunk chunk1 ->
+      valid_access m chunk1 ofs ->
+      valid_access m chunk2 ofs.
+  Proof.
+    intros. inv H1. rewrite H in H2. constructor; auto.
+    eapply Z.divide_trans; eauto. eapply align_le_divides; eauto.
+  Qed.
+
+  Lemma valid_access_dec:
+    forall m chunk ofs,
+      {valid_access m chunk ofs} + {~ valid_access m chunk ofs}.
+  Proof.
+    intros.
+    destruct (range_perm_dec m ofs (ofs + size_chunk chunk) Live).
+    destruct (Zdivide_dec (align_chunk chunk) ofs).
+    left; constructor; auto.
+    right; red; intro V; inv V; contradiction.
+    right; red; intro V; inv V; contradiction.
+  Defined.
   
   Definition allowed_access (m: mem) (chunk: memory_chunk) (ofs: Z) : Prop :=
     range_perm_neg m ofs (ofs + size_chunk chunk) Dead.
@@ -208,6 +271,41 @@ Module Mem (P:Policy).
     intros. destruct (Zdivide_dec (align_chunk chunk) ofs); auto.
   Qed.
   
+(*  Lemma valid_access_allowed:
+    forall m chunk ofs,
+      valid_access m chunk ofs ->
+      allowed_access m chunk ofs.
+  Proof.
+    unfold valid_access, allowed_access. intros.
+    destruct H. split; auto.
+    unfold range_perm in *. unfold range_perm_neg. intros.
+    specialize H with ofs0. apply H in H1. intro.
+    unfold perm in *. rewrite H1 in H2. discriminate.
+  Qed.*)
+
+  (** C allows pointers one past the last element of an array.  These are not
+      valid according to the previously defined [valid_pointer]. The property
+      [weak_valid_pointer m ofs] holds if address [b, ofs] is a valid pointer
+      in [m], or a pointer one past a valid block in [m].  *)
+  
+(*  Definition weak_valid_pointer (m: mem) (ofs: Z) :=
+    valid_pointer m ofs || valid_pointer m (ofs - 1).
+
+Lemma weak_valid_pointer_spec:
+  forall m ofs,
+  weak_valid_pointer m ofs = true <->
+    valid_pointer m ofs = true \/ valid_pointer m (ofs - 1) = true.
+Proof.
+  intros. unfold weak_valid_pointer. now rewrite orb_true_iff.
+Qed.
+Lemma valid_pointer_implies:
+  forall m ofs,
+  valid_pointer m ofs = true -> weak_valid_pointer m ofs = true.
+Proof.
+  intros. apply weak_valid_pointer_spec. auto.
+Qed.
+ *)
+  
 (** * Operations over memory stores *)
 
 (** The initial store *)
@@ -219,6 +317,11 @@ Module Mem (P:Policy).
           (fun ofs => if init_dead ofs then Dead else MostlyDead)
           []
   .
+
+  (** Freeing a block between the given bounds.
+      Return the updated memory state where the given range of the given block
+      has been invalidated: future reads and writes to this
+      range will fail.  Requires freeable permission on the given range. *)
 
   Remark region_eq_dec :
     forall (r1 r2:Z*Z%type),
@@ -431,6 +534,124 @@ Module Mem (P:Policy).
     destruct (init_dead ofs); intro; discriminate.
   Qed.
 
+  Theorem valid_access_empty: forall chunk ofs, ~valid_access empty chunk ofs.
+  Proof.
+    intros. red; intros. elim (perm_empty ofs). apply H.
+    generalize (size_chunk_pos chunk); lia.
+  Qed.
+
+  (** ** Properties related to [load] *)
+
+(*  Theorem allowed_access_load:
+    forall m chunk ofs,
+      allowed_access m chunk ofs ->
+      exists v, load chunk m ofs = MemorySuccess v.
+  Proof.
+    intros. econstructor. unfold load. rewrite pred_dec_true; eauto.
+  Qed.*)
+
+(*  Theorem valid_access_load:
+    forall m chunk ofs,
+      valid_access m chunk ofs ->
+      exists v, load chunk m ofs = MemorySuccess v.
+  Proof.
+    intros. econstructor. unfold load.
+    rewrite pred_dec_true; eauto. eapply valid_access_allowed. auto.
+  Qed.*)
+
+(*  Theorem load_allowed_access:
+    forall m chunk ofs v,
+      load chunk m ofs = MemorySuccess v ->
+      allowed_access m chunk ofs.
+  Proof.
+    intros until v. unfold load.
+    destruct (allowed_access_dec m chunk ofs); intros.
+    auto.
+    inv H.
+  Qed.*)
+
+(*  Lemma load_result:
+    forall chunk m ofs v,
+      load chunk m ofs = MemorySuccess v ->
+      v = decode_val chunk (map (fun x => fst x) (getN (size_chunk_nat chunk) ofs (m.(mem_contents)))).
+  Proof.
+    intros until v. unfold load.
+    destruct (allowed_access_dec m chunk ofs); intros.
+    congruence.
+    congruence.
+  Qed.*)
+
+(*  Local Hint Resolve load_allowed_access valid_access_load: mem.*)
+
+  Theorem load_type:
+    forall m chunk ofs v vt,
+      load chunk m ofs = MemorySuccess (v,vt) ->
+      Val.has_type v (type_of_chunk chunk).
+  Admitted.
+  (*Proof.
+    intros. exploit load_result; eauto; intros. rewrite H0.
+    apply decode_val_type.
+    Qed.*)
+
+  Theorem load_rettype:
+    forall m chunk ofs v vt,
+      load chunk m ofs = MemorySuccess (v,vt) ->
+      Val.has_rettype v (rettype_of_chunk chunk).
+  Admitted.
+  (*Proof.
+    intros. exploit load_result; eauto; intros. rewrite H0.
+    apply decode_val_rettype.
+    Qed.*)
+
+  Theorem load_cast:
+    forall m chunk ofs v vt,
+      load chunk m ofs = MemorySuccess (v,vt) ->
+      match chunk with
+      | Mint8signed => v = Val.sign_ext 8 v
+      | Mint8unsigned => v = Val.zero_ext 8 v
+      | Mint16signed => v = Val.sign_ext 16 v
+      | Mint16unsigned => v = Val.zero_ext 16 v
+      | _ => True
+      end.
+  Admitted.
+(*Proof.
+  intros. exploit load_result; eauto.
+  set (l := getN (size_chunk_nat chunk) ofs m.(mem_contents)#b).
+  intros. subst v. apply decode_val_cast.
+Qed.*)
+
+(*Theorem load_int8_signed_unsigned:
+  forall m ofs,
+  load Mint8signed m ofs = opt_atom_map (Val.sign_ext 8) (load Mint8unsigned m ofs).
+Admitted.
+(*Proof.
+  intros. unfold load.
+  change (size_chunk_nat Mint8signed) with (size_chunk_nat Mint8unsigned).
+  set (cl := getN (size_chunk_nat Mint8unsigned) ofs m.(mem_contents)#b).
+  destruct (allowed_access_dec m Mint8signed ofs).
+  rewrite pred_dec_true; auto. unfold decode_val.
+  destruct (proj_bytes cl); auto.
+  simpl. decEq. decEq. rewrite Int.sign_ext_zero_ext. auto. compute; auto.
+  rewrite pred_dec_false; auto.
+Qed.*)
+
+Theorem load_int16_signed_unsigned:
+  forall m ofs,
+  load Mint16signed m ofs = opt_atom_map (Val.sign_ext 16) (load Mint16unsigned m ofs).
+Admitted.
+(*Proof.
+  intros. unfold load.
+  change (size_chunk_nat Mint16signed) with (size_chunk_nat Mint16unsigned).
+  set (cl := getN (size_chunk_nat Mint16unsigned) ofs m.(mem_contents)#b).
+  destruct (allowed_access_dec m Mint16signed ofs).
+  rewrite pred_dec_true; auto. unfold decode_val.
+  destruct (proj_bytes cl); auto.
+  simpl. decEq. decEq. rewrite Int.sign_ext_zero_ext. auto. compute; auto.
+  rewrite pred_dec_false; auto.
+Qed.*)
+*)
+(** ** Properties related to [loadbytes] *)
+
 Theorem range_perm_loadbytes:
   forall m ofs len,
   range_perm_neg m ofs (ofs + len) Dead ->
@@ -439,14 +660,14 @@ Proof.
   intros. econstructor. unfold loadbytes. rewrite pred_dec_true; eauto.
 Qed.
 
-(*Axiom range_perm_loadbytes_live:
+Axiom range_perm_loadbytes_live:
   forall m ofs len,
   range_perm m ofs (ofs + len) Live ->
   exists bytes, loadbytes m ofs len = MemorySuccess bytes.
 Axiom range_perm_loadbytes_md:
   forall m ofs len,
   range_perm m ofs (ofs + len) MostlyDead ->
-  exists bytes, loadbytes m ofs len = MemorySuccess bytes.*)
+  exists bytes, loadbytes m ofs len = MemorySuccess bytes.
 
 Theorem loadbytes_range_perm:
   forall m ofs len bytes,
@@ -458,11 +679,49 @@ Proof.
   congruence.
 Qed.
 
+(*Theorem loadbytes_load:
+  forall chunk m ofs bytes,
+  loadbytes m ofs (size_chunk chunk) = MemorySuccess bytes ->
+  (align_chunk chunk | ofs) ->
+  load chunk m ofs = MemorySuccess(decode_val chunk bytes).
+Proof.
+  unfold loadbytes, load; intros.
+  destruct (range_perm_neg_dec m ofs (ofs + size_chunk chunk) Dead);
+  try congruence.
+  inv H. rewrite pred_dec_true. auto.
+  split; auto.
+Qed.*)
+
+Theorem load_loadbytes:
+  forall chunk m ofs v,
+  load chunk m ofs = MemorySuccess v ->
+  exists bytes, loadbytes m ofs (size_chunk chunk) = MemorySuccess bytes
+             /\ v = decode_val chunk bytes.
+Admitted.
+(*Proof.
+  intros. exploit load_allowed_access; eauto. intros [A B].
+  exploit load_result; eauto. intros.
+  exists (getN (size_chunk_nat chunk) ofs m.(mem_contents)#b); split.
+  unfold loadbytes. rewrite pred_dec_true; auto.
+  auto.
+Qed.*)
+
 Lemma getN_length:
   forall c n p, length (getN n p c) = n.
 Proof.
   induction n; simpl; intros. auto. decEq; auto.
 Qed.
+
+Theorem loadbytes_length:
+  forall m ofs n bytes,
+  loadbytes m ofs n = MemorySuccess bytes ->
+  length bytes = Z.to_nat n.
+Admitted.
+(*Proof.
+  unfold loadbytes; intros.
+  destruct (range_perm_neg_dec m ofs (ofs + n) Dead); try congruence.
+  inv H. apply getN_length.
+Qed.*)
 
 Theorem loadbytes_empty:
   forall m ofs n,
@@ -483,6 +742,639 @@ Proof.
   auto.
 Qed.
 
+Theorem loadbytes_concat:
+  forall m ofs n1 n2 bytes1 bytes2,
+  loadbytes m ofs n1 = MemorySuccess bytes1 ->
+  loadbytes m (ofs + n1) n2 = MemorySuccess bytes2 ->
+  n1 >= 0 -> n2 >= 0 ->
+  loadbytes m ofs (n1 + n2) = MemorySuccess(bytes1 ++ bytes2).
+Admitted.
+(*Proof.
+  unfold loadbytes; intros.
+  destruct (range_perm_neg_dec m ofs (ofs + n1) Dead); try congruence.
+  destruct (range_perm_neg_dec m (ofs + n1) (ofs + n1 + n2) Dead); try congruence.
+  rewrite pred_dec_true. rewrite Z2Nat.inj_add by lia.
+  rewrite getN_concat. rewrite Z2Nat.id by lia.
+  congruence.
+  red; intros.
+  assert (ofs0 < ofs + n1 \/ ofs0 >= ofs + n1) by lia.
+  destruct H4. apply r; lia. apply r0; lia.
+Qed.*)
+
+Theorem loadbytes_split:
+  forall m ofs n1 n2 bytes,
+  loadbytes m ofs (n1 + n2) = MemorySuccess bytes ->
+  n1 >= 0 -> n2 >= 0 ->
+  exists bytes1, exists bytes2,
+     loadbytes m ofs n1 = MemorySuccess bytes1
+  /\ loadbytes m (ofs + n1) n2 = MemorySuccess bytes2
+  /\ bytes = bytes1 ++ bytes2.
+Admitted.
+(*Proof.
+  unfold loadbytes; intros.
+  destruct (range_perm_neg_dec m ofs (ofs + (n1 + n2)) Dead);
+  try congruence.
+  rewrite Z2Nat.inj_add in H by lia. rewrite getN_concat in H.
+  rewrite Z2Nat.id in H by lia.
+  repeat rewrite pred_dec_true.
+  econstructor; econstructor.
+  split. reflexivity. split. reflexivity. congruence.
+  red; intros; apply r; lia.
+  red; intros; apply r; lia.
+Qed.*)
+
+Theorem load_rep:
+ forall ch m1 m2 ofs v1 v2,
+  (forall z, 0 <= z < size_chunk ch -> ZMap.get (ofs + z) m1.(mem_contents)= ZMap.get (ofs + z) m2.(mem_contents)) ->
+  load ch m1 ofs = MemorySuccess v1 ->
+  load ch m2 ofs = MemorySuccess v2 ->
+  v1 = v2.
+Admitted.
+(*Proof.
+  intros.
+  apply load_result in H0.
+  apply load_result in H1.
+  subst.
+  f_equal.
+  rewrite size_chunk_conv in H.
+  remember (size_chunk_nat ch) as n; clear Heqn.
+  revert ofs H; induction n; intros; simpl; auto.
+  f_equal.
+  rewrite Nat2Z.inj_succ in H.
+  replace ofs with (ofs+0) by lia.
+  apply H; lia.
+  apply IHn.
+  intros.
+  rewrite <- Z.add_assoc.
+  apply H.
+  rewrite Nat2Z.inj_succ. lia.
+Qed.*)
+
+(*Theorem load_int64_split:
+  forall m ofs v,
+  load Mint64 m ofs = Some v -> Archi.ptr64 = false ->
+  exists v1 v2,
+     load Mint32 m ofs = Some (if Archi.big_endian then v1 else v2)
+  /\ load Mint32 m (ofs + 4) = Some (if Archi.big_endian then v2 else v1)
+  /\ Val.lessdef v (Val.longofwords v1 v2).
+Proof.
+  intros.
+  exploit load_allowed_access; eauto. intros [A B]. simpl in *.
+  exploit load_loadbytes. eexact H. simpl. intros [bytes [LEQ]].
+  change 8 with (4 + 4) in LB.
+  exploit loadbytes_split. eexact LB. lia. lia.
+  intros (bytes1 & bytes2 & LB1 & LB2 & APP).
+  change 4 with (size_chunk Mint32) in LB1.
+  exploit loadbytes_load. eexact LB1.
+  simpl. apply Z.divide_trans with 8; auto. exists 2; auto.
+  intros L1.
+  change 4 with (size_chunk Mint32) in LB2.
+  exploit loadbytes_load. eexact LB2.
+  simpl. apply Z.divide_add_r. apply Z.divide_trans with 8; auto. exists 2; auto. exists 1; auto.
+  intros L2.
+  exists (decode_val Mint32 (if Archi.big_endian then bytes1 else bytes2));
+  exists (decode_val Mint32 (if Archi.big_endian then bytes2 else bytes1)).
+  split. destruct Archi.big_endian; auto.
+  split. destruct Archi.big_endian; auto.
+  rewrite EQ. rewrite APP. apply decode_val_int64; auto.
+  erewrite loadbytes_length; eauto. reflexivity.
+  erewrite loadbytes_length; eauto. reflexivity.
+Qed.*)
+
+Lemma addressing_int64_split:
+  forall i,
+  Archi.ptr64 = false ->
+  (8 | Ptrofs.unsigned i) ->
+  Ptrofs.unsigned (Ptrofs.add i (Ptrofs.of_int (Int.repr 4))) = Ptrofs.unsigned i + 4.
+Proof.
+  intros.
+  rewrite Ptrofs.add_unsigned.
+  replace (Ptrofs.unsigned (Ptrofs.of_int (Int.repr 4))) with (Int.unsigned (Int.repr 4))
+    by (symmetry; apply Ptrofs.agree32_of_int; auto).
+  change (Int.unsigned (Int.repr 4)) with 4.
+  apply Ptrofs.unsigned_repr.
+  exploit (Zdivide_interval (Ptrofs.unsigned i) Ptrofs.modulus 8).
+  lia. apply Ptrofs.unsigned_range. auto.
+  exists (two_p (Ptrofs.zwordsize - 3)).
+  unfold Ptrofs.modulus, Ptrofs.zwordsize, Ptrofs.wordsize.
+  unfold Wordsize_Ptrofs.wordsize. destruct Archi.ptr64; reflexivity.
+  unfold Ptrofs.max_unsigned. lia.
+Qed.
+
+(*Theorem loadv_int64_split:
+  forall m a v,
+  loadv Mint64 m a = Some v -> Archi.ptr64 = false ->
+  exists v1 v2,
+     loadv Mint32 m a = Some (if Archi.big_endian then v1 else v2)
+  /\ loadv Mint32 m (Val.add a (Vint (Int.repr 4))) = Some (if Archi.big_endian then v2 else v1)
+  /\ Val.lessdef v (Val.longofwords v1 v2).
+Proof.
+  intros. destruct a; simpl in H; inv H.
+  exploit load_int64_split; eauto.
+  intros (v1 & v2 & L1 & L2 & EQ).
+  unfold Val.add; rewrite H0.
+  assert (NV: Ptrofs.unsigned (Ptrofs.add i (Ptrofs.of_int (Int.repr 4))) = Ptrofs.unsigned i + 4).
+  { apply addressing_int64_split; auto.
+    exploit load_allowed_access. eexact H2. intros [P Q]. auto. }
+  exists v1, v2.
+Opaque Ptrofs.repr.
+  split. auto.
+  split. simpl. rewrite NV. auto.
+  auto.
+Qed.*)
+
+(** ** Properties related to [store] *)
+
+(*Theorem valid_access_store:
+  forall m1 chunk ofs a lts,
+  valid_access m1 chunk ofs ->
+  { m2: mem | store chunk m1 ofs a lts = MemorySuccess m2 }.
+Proof.
+  intros.
+  unfold store.
+  destruct (allowed_access_dec m1 chunk ofs).
+  eauto.
+  apply valid_access_allowed in H.
+  contradiction.
+Defined.*)
+
+(*Local Hint Resolve valid_access_store: mem.*)
+
+(*Theorem allowed_access_store:
+  forall m1 chunk ofs v vt lts,
+  allowed_access m1 chunk ofs ->
+  { m2: mem | store chunk m1 ofs (v,vt) lts = MemorySuccess m2 }.
+Proof.
+  intros.
+  unfold store.
+  destruct (allowed_access_dec m1 chunk ofs).
+  eauto.
+  contradiction.
+Defined.*)
+
+(*Local Hint Resolve allowed_access_store: mem.*)
+
+Axiom disallowed_access_store:
+  forall m1 chunk ofs v vt lts,
+  ~ allowed_access m1 chunk ofs ->
+  store chunk m1 ofs (v,vt) lts = MemoryFail "" (PrivateStore ofs).
+
+(*Local Hint Resolve allowed_access_store: mem.*)
+
+Section STORE.
+Variable chunk: memory_chunk.
+Variable m1: mem.
+Variable ofs: Z.
+Variable v: val.
+Variable vt: tag.
+Variable lts: list tag.
+Variable m2: mem.
+Hypothesis STORE: store chunk m1 ofs (v,vt) lts = MemorySuccess m2.
+
+(*Lemma store_access: mem_access m2 = mem_access m1.
+Proof.
+  unfold store in STORE. destruct ( allowed_access_dec m1 chunk ofs); inv STORE.
+  auto.
+Qed.
+
+Lemma store_mem_contents:
+  mem_contents m2 = setN (merge_vals_tags (encode_val chunk (v,vt)) lts) ofs (m1.(mem_contents)).
+Proof.
+  unfold store in STORE. destruct (allowed_access_dec m1 chunk ofs); inv STORE. simpl.
+  auto.
+Qed.
+
+Theorem perm_store_1:
+  forall ofs' p, perm m1 ofs' p -> perm m2 ofs' p.
+Proof.
+  intros.
+ unfold perm in *. unfold get_perm in *. rewrite store_access; auto.
+Qed.
+
+Theorem perm_store_2:
+  forall ofs' p, perm m2 ofs' p -> perm m1 ofs' p.
+Proof.
+  intros. unfold perm in *. unfold get_perm in *. rewrite store_access in H; auto.
+Qed.
+
+Local Hint Resolve perm_store_1 perm_store_2: mem.
+
+Theorem store_valid_block_1:
+  forall ofs', valid_addr m1 ofs' -> valid_addr m2 ofs'.
+Proof.
+  unfold valid_addr; intros. destruct H as [lo [hi H]]. exists lo. exists hi.
+  unfold store in *. destruct (allowed_access_dec m1 chunk ofs); inv STORE.
+  simpl. auto.
+Qed.
+
+Theorem store_valid_block_2:
+  forall ofs', valid_addr m2 ofs' -> valid_addr m1 ofs'.
+Proof.
+  unfold valid_addr; intros. destruct H as [lo [hi H]]. exists lo. exists hi.
+  unfold store in *. destruct (allowed_access_dec m1 chunk ofs); inv STORE.
+  simpl. auto.
+Qed.
+
+Local Hint Resolve store_valid_block_1 store_valid_block_2: mem.
+
+Theorem store_valid_access_1:
+  forall chunk' ofs',
+    valid_access m1 chunk' ofs' -> valid_access m2 chunk' ofs'.
+Proof.
+  intros. inv H. constructor; try red; auto with mem.
+Qed.
+
+Theorem store_valid_access_2:
+  forall chunk' ofs',
+    valid_access m2 chunk' ofs' -> valid_access m1 chunk' ofs'.
+Proof.
+  intros. inv H. constructor; try red; auto with mem.
+Qed.
+
+Theorem store_allowed_access_1:
+  forall chunk' ofs',
+    allowed_access m1 chunk' ofs' -> allowed_access m2 chunk' ofs'.
+Admitted.
+(*Proof.
+  intros. inv H. constructor; try red; auto with mem.
+Qed.*)
+
+Theorem store_allowed_access_2:
+  forall chunk' ofs',
+    allowed_access m2 chunk' ofs' -> allowed_access m1 chunk' ofs'.
+Admitted.
+(*Proof.
+  intros. inv H. constructor; try red; auto with mem.
+Qed.*)
+
+Theorem store_allowed_access_3:
+  allowed_access m1 chunk ofs.
+Proof.
+  unfold store in STORE. destruct (allowed_access_dec m1 chunk ofs).
+  auto.
+  congruence.
+Qed.
+
+Theorem store_allowed_access_4:
+  forall chunk' ofs',
+    ~allowed_access m1 chunk' ofs' -> ~allowed_access m2 chunk' ofs'.
+Admitted.
+
+Local Hint Resolve store_allowed_access_1 store_allowed_access_2 store_allowed_access_3 store_allowed_access_4: mem.
+
+Theorem load_store_similar:
+  forall chunk',
+  size_chunk chunk' = size_chunk chunk ->
+  align_chunk chunk' <= align_chunk chunk ->
+  exists v' t', load chunk' m2 ofs = MemorySuccess (v',t') /\ decode_encode_val v chunk chunk' v'.
+Admitted.
+(*Proof.
+  intros.
+  exploit (allowed_access_load m2 chunk' b).
+    eapply allowed_access_compat. symmetry; eauto. auto. eauto with mem.
+  intros [v' LOAD].
+  exists v'; split; auto.
+  exploit load_result; eauto. intros B.
+  rewrite B. rewrite store_mem_contents; simpl.
+  rewrite PMap.gss.
+  replace (size_chunk_nat chunk') with (length (encode_val chunk v)).
+  rewrite getN_setN_same. apply decode_encode_val_general.
+  rewrite encode_val_length. repeat rewrite size_chunk_conv in H.
+  apply Nat2Z.inj; auto.
+Qed.*)
+
+Theorem load_store_similar_2:
+  forall chunk',
+  size_chunk chunk' = size_chunk chunk ->
+  align_chunk chunk' <= align_chunk chunk ->
+  type_of_chunk chunk' = type_of_chunk chunk ->
+  load chunk' m2 ofs = MemorySuccess (Val.load_result chunk' v, vt).
+Admitted.
+(*Proof.
+  intros. destruct (load_store_similar chunk') as [v' [A B]]; auto.
+  rewrite A. decEq. eapply decode_encode_val_similar with (chunk1 := chunk); eauto.
+Qed.*)
+
+Theorem load_store_same:
+  load chunk m2 ofs = MemorySuccess (Val.load_result chunk v, vt).
+Proof.
+  apply load_store_similar_2; auto. lia.
+Qed.
+
+Theorem load_store_other:
+  forall chunk' ofs',
+    ofs' + size_chunk chunk' <= ofs
+    \/ ofs + size_chunk chunk <= ofs' ->
+    load chunk' m2 ofs' = load chunk' m1 ofs'.
+Admitted.
+(*Proof.
+  intros. unfold load.
+  destruct (allowed_access_dec m1 chunk' ofs').
+  rewrite pred_dec_true.
+  decEq. decEq. rewrite store_mem_contents; simpl.
+  rewrite PMap.gsspec. destruct (peq b). subst b'.
+  apply getN_setN_outside. rewrite encode_val_length. repeat rewrite <- size_chunk_conv.
+  intuition.
+  auto.
+  eauto with mem.
+  rewrite pred_dec_false. auto.
+  eauto with mem.
+Qed.*)
+
+Theorem loadbytes_store_same:
+  loadbytes m2 ofs (size_chunk chunk) = MemorySuccess(encode_val chunk (v, vt)).
+Admitted.
+(*Proof.
+  intros.
+  assert (allowed_access m2 chunk ofs) by eauto with mem.
+  unfold loadbytes. rewrite pred_dec_true. rewrite store_mem_contents; simpl.
+  rewrite PMap.gss.
+  replace (Z.to_nat (size_chunk chunk)) with (length (encode_val chunk v)).
+  rewrite getN_setN_same. auto.
+  rewrite encode_val_length. auto.
+  apply H.
+Qed.*)
+
+Theorem loadbytes_store_other:
+  forall ofs' n,
+    n <= 0
+    \/ ofs' + n <= ofs
+    \/ ofs + size_chunk chunk <= ofs' ->
+    loadbytes m2 ofs' n = loadbytes m1 ofs' n.
+Admitted.
+(*Proof.
+  intros. unfold loadbytes.
+  destruct (range_perm_neg_dec m1 ofs' (ofs' + n) Dead).
+  rewrite pred_dec_true.
+  decEq. rewrite store_mem_contents; simpl.
+  rewrite PMap.gsspec. destruct (peq b). subst b'.
+  destruct H. congruence.
+  destruct (zle n 0) as [z | n0].
+  rewrite (Z_to_nat_neg _ z). auto.
+  destruct H. extlia.
+  apply getN_setN_outside. rewrite encode_val_length. rewrite <- size_chunk_conv.
+  rewrite Z2Nat.id. auto. lia.
+  auto.
+  red; intros. assert (~ perm m1 ofs0 Dead) by admit. eauto with mem.
+  rewrite pred_dec_false. auto.
+  red; intro; elim n0; red; intros. admit. (*; eauto with mem.*)
+Admitted.*)
+
+Lemma setN_in:
+  forall vl p q c,
+  p <= q < p + Z.of_nat (length vl) ->
+  In (ZMap.get q (setN vl p c)) vl.
+Proof.
+  induction vl; intros.
+  simpl in H. extlia.
+  simpl length in H. rewrite Nat2Z.inj_succ in H. simpl.
+  destruct (zeq p q). subst q. rewrite setN_outside. rewrite ZMap.gss.
+  auto with coqlib. lia.
+  right. apply IHvl. lia.
+Qed.
+
+Lemma getN_in:
+  forall c q n p,
+  p <= q < p + Z.of_nat n ->
+  In (ZMap.get q c) (getN n p c).
+Proof.
+  induction n; intros.
+  simpl in H; extlia.
+  rewrite Nat2Z.inj_succ in H. simpl. destruct (zeq p q).
+  subst q. auto.
+  right. apply IHn. lia.
+Qed.
+*)
+End STORE.
+
+(*Local Hint Resolve perm_store_1 perm_store_2: mem.
+Local Hint Resolve store_valid_block_1 store_valid_block_2: mem.
+Local Hint Resolve store_allowed_access_1 store_allowed_access_2
+             store_allowed_access_3 store_allowed_access_4: mem.*)
+
+(*Lemma load_store_overlap:
+  forall chunk m1 ofs v vt lts m2 chunk' ofs' v',
+  store chunk m1 ofs v vt lts = Some m2 ->
+  load chunk' m2 ofs' = Some v' ->
+  ofs' + size_chunk chunk' > ofs ->
+  ofs + size_chunk chunk > ofs' ->
+  exists mv1 mvl mv1' mvl',
+      shape_encoding chunk v (mv1 :: mvl)
+  /\  shape_decoding chunk' (mv1' :: mvl') v'
+  /\  (   (ofs' = ofs /\ mv1' = mv1)
+       \/ (ofs' > ofs /\ In mv1' mvl)
+       \/ (ofs' < ofs /\ In mv1 mvl')).
+Admitted.
+Proof.
+  intros.
+  exploit load_result; eauto. erewrite store_mem_contents by eauto; simpl.
+  rewrite PMap.gss.
+  set (c := (mem_contents m1)#b). intros V'.
+  destruct (size_chunk_nat_pos chunk) as [sz SIZE].
+  destruct (size_chunk_nat_pos chunk') as [sz' SIZE'].
+  destruct (encode_val chunk v) as [ | mv1 mvl] eqn:ENC.
+  generalize (encode_val_length chunk v); rewrite ENC; simpl; congruence.
+  set (c' := setN (mv1::mvl) ofs c) in *.
+  exists mv1, mvl, (ZMap.get ofs' c'), (getN sz' (ofs' + 1) c').
+  split. rewrite <- ENC. apply encode_val_shape.
+  split. rewrite V', SIZE'. apply decode_val_shape.
+  destruct (zeq ofs' ofs).
+- subst ofs'. left; split. auto. unfold c'. simpl.
+  rewrite setN_outside by lia. apply ZMap.gss.
+- right. destruct (zlt ofs ofs').
+(* If ofs < ofs':  the load reads (at ofs') a continuation byte from the write.
+       ofs   ofs'   ofs+|chunk|
+        [-------------------]       write
+             [-------------------]  read
+*)
++ left; split. lia. unfold c'. simpl. apply setN_in.
+  assert (Z.of_nat (length (mv1 :: mvl)) = size_chunk chunk).
+  { rewrite <- ENC; rewrite encode_val_length. rewrite size_chunk_conv; auto. }
+  simpl length in H3. rewrite Nat2Z.inj_succ in H3. lia.
+(* If ofs > ofs':  the load reads (at ofs) the first byte from the write.
+       ofs'   ofs   ofs'+|chunk'|
+               [-------------------]  write
+         [----------------]           read
+*)
++ right; split. lia. replace mv1 with (ZMap.get ofs c').
+  apply getN_in.
+  assert (size_chunk chunk' = Z.succ (Z.of_nat sz')).
+  { rewrite size_chunk_conv. rewrite SIZE'. rewrite Nat2Z.inj_succ; auto. }
+  lia.
+  unfold c'. simpl. rewrite setN_outside by lia. apply ZMap.gss.
+Qed.*)
+
+Definition compat_pointer_chunks (chunk1 chunk2: memory_chunk) : Prop :=
+  match chunk1, chunk2 with
+  | (Mint32 | Many32), (Mint32 | Many32) => True
+  | (Mint64 | Many64), (Mint64 | Many64) => True
+  | _, _ => False
+  end.
+
+(*Lemma compat_pointer_chunks_true:
+  forall chunk1 chunk2,
+  (chunk1 = Mint32 \/ chunk1 = Many32 \/ chunk1 = Mint64 \/ chunk1 = Many64) ->
+  (chunk2 = Mint32 \/ chunk2 = Many32 \/ chunk2 = Mint64 \/ chunk2 = Many64) ->
+  quantity_chunk chunk1 = quantity_chunk chunk2 ->
+  compat_pointer_chunks chunk1 chunk2.
+Proof.
+  intros. destruct H as [P|[P|[P|P]]]; destruct H0 as [Q|[Q|[Q|Q]]];
+  subst; red; auto; discriminate.
+Qed.*)
+
+Theorem load_pointer_store:
+  forall chunk m1 ofs v pt lts m2 chunk' ofs' v_v_o pt',
+  store chunk m1 ofs (v,pt) lts = MemorySuccess m2 ->
+  load chunk' m2 ofs' = MemorySuccess(Vint v_v_o, pt') ->
+  (v = Vint v_v_o /\ compat_pointer_chunks chunk chunk' /\ ofs' = ofs)
+  \/ (ofs' + size_chunk chunk' <= ofs \/ ofs + size_chunk chunk <= ofs').
+Admitted.
+(*Proof.
+  intros.
+  destruct (peq b); auto. subst b'.
+  destruct (zle (ofs' + size_chunk chunk') ofs); auto.
+  destruct (zle (ofs + size_chunk chunk) ofs'); auto.
+  exploit load_store_overlap; eauto.
+  intros (mv1 & mvl & mv1' & mvl' & ENC & DEC & CASES).
+  inv DEC; try contradiction.
+  destruct CASES as [(A & B) | [(A & B) | (A & B)]].
+- (* Same offset *)
+  subst. inv ENC.
+  assert (chunk = Mint32 \/ chunk = Many32 \/ chunk = Mint64 \/ chunk = Many64)
+  by (destruct chunk; auto || contradiction).
+  left; split. rewrite H3.
+  destruct H4 as [P|[P|[P|P]]]; subst chunk'; destruct v0; simpl in H3;
+  try congruence; destruct Archi.ptr64; congruence.
+  split. apply compat_pointer_chunks_true; auto.
+  auto.
+- (* ofs' > ofs *)
+  inv ENC.
+  + exploit H10; eauto. intros (j & P & Q). inv P. congruence.
+  + exploit H8; eauto. intros (n & P); congruence.
+  + exploit H2; eauto. congruence.
+- (* ofs' < ofs *)
+  exploit H7; eauto. intros (j & P & Q). subst mv1. inv ENC. congruence.
+Qed.*)
+
+Theorem load_store_pointer_overlap:
+  forall chunk m1 ofs v_v_o m2 chunk' ofs' v pt lts,
+  store chunk m1 ofs (Vint v_v_o, pt) lts = MemorySuccess m2 ->
+  load chunk' m2 ofs' = MemorySuccess v ->
+  ofs' <> ofs ->
+  ofs' + size_chunk chunk' > ofs ->
+  ofs + size_chunk chunk > ofs' ->
+  v = (Vundef, def_tag).
+Admitted.
+(*Proof.
+  intros.
+  exploit load_store_overlap; eauto.
+  intros (mv1 & mvl & mv1' & mvl' & ENC & DEC & CASES).
+  destruct CASES as [(A & B) | [(A & B) | (A & B)]].
+- congruence.
+- inv ENC.
+  + exploit H9; eauto. intros (j & P & Q). subst mv1'. inv DEC. congruence. auto.
+  + contradiction.
+  + exploit H5; eauto. intros; subst. inv DEC; auto.
+- inv DEC.
+  + exploit H10; eauto. intros (j & P & Q). subst mv1. inv ENC. congruence.
+  + exploit H8; eauto. intros (n & P). subst mv1. inv ENC. contradiction.
+  + auto.
+Qed.*)
+
+Theorem load_store_pointer_mismatch:
+  forall chunk m1 ofs v_v_o m2 chunk' v pt lts,
+  store chunk m1 ofs (Vint v_v_o, pt) lts = MemorySuccess m2 ->
+  load chunk' m2 ofs = MemorySuccess v ->
+  ~compat_pointer_chunks chunk chunk' ->
+  v = (Vundef, def_tag).
+Admitted.
+(*Proof.
+  intros.
+  exploit load_store_overlap; eauto.
+  generalize (size_chunk_pos chunk'); lia.
+  generalize (size_chunk_pos chunk); lia.
+  intros (mv1 & mvl & mv1' & mvl' & ENC & DEC & CASES).
+  destruct CASES as [(A & B) | [(A & B) | (A & B)]]; try extlia.
+  inv ENC; inv DEC; auto.
+- elim H1. apply compat_pointer_chunks_true; auto.
+- contradiction.
+Qed.*)
+
+Lemma store_similar_chunks:
+  forall chunk1 chunk2 v1 v2 lts1 lts2 m ofs,
+  encode_val chunk1 v1 = encode_val chunk2 v2 ->
+  align_chunk chunk1 = align_chunk chunk2 ->
+  store chunk1 m ofs v1 lts1 = store chunk2 m ofs v2 lts2.
+Admitted.
+(*Proof.
+  intros. unfold store.
+  assert (size_chunk chunk1 = size_chunk chunk2).
+    repeat rewrite size_chunk_conv.
+    rewrite <- (encode_val_length chunk1 v1).
+    rewrite <- (encode_val_length chunk2 v2).
+    congruence.
+  unfold store.
+  destruct (allowed_access_dec m chunk1 ofs);
+  destruct (allowed_access_dec m chunk2 ofs); auto.
+  f_equal. apply mkmem_ext; auto. congruence.
+  elim n. apply allowed_access_compat with chunk1; auto. lia.
+  elim n. apply allowed_access_compat with chunk2; auto. lia.
+Qed.*)
+
+Theorem store_signed_unsigned_8:
+  forall m ofs v vt lts,
+  store Mint8signed m ofs (v,vt) lts = store Mint8unsigned m ofs (v,vt) lts.
+Proof. intros. apply store_similar_chunks. apply encode_val_int8_signed_unsigned. auto. Qed.
+
+Theorem store_signed_unsigned_16:
+  forall m ofs v vt lts,
+  store Mint16signed m ofs (v,vt) lts = store Mint16unsigned m ofs (v,vt) lts.
+Proof. intros. apply store_similar_chunks. apply encode_val_int16_signed_unsigned. auto. Qed.
+
+Theorem store_int8_zero_ext:
+  forall m ofs n vt lts,
+  store Mint8unsigned m ofs (Vint (Int.zero_ext 8 n), vt) lts =
+  store Mint8unsigned m ofs (Vint n, vt) lts.
+Proof. intros. apply store_similar_chunks. apply encode_val_int8_zero_ext. auto. Qed.
+
+Theorem store_int8_sign_ext:
+  forall m ofs n vt lts,
+  store Mint8signed m ofs (Vint (Int.sign_ext 8 n), vt) lts =
+  store Mint8signed m ofs (Vint n, vt) lts.
+Proof. intros. apply store_similar_chunks. apply encode_val_int8_sign_ext. auto. Qed.
+
+Theorem store_int16_zero_ext:
+  forall m ofs n vt lts,
+  store Mint16unsigned m ofs (Vint (Int.zero_ext 16 n), vt) lts =
+  store Mint16unsigned m ofs (Vint n, vt) lts.
+Proof. intros. apply store_similar_chunks. apply encode_val_int16_zero_ext. auto. Qed.
+
+Theorem store_int16_sign_ext:
+  forall m ofs n vt lts,
+  store Mint16signed m ofs (Vint (Int.sign_ext 16 n), vt) lts =
+  store Mint16signed m ofs (Vint n, vt) lts.
+Proof. intros. apply store_similar_chunks. apply encode_val_int16_sign_ext. auto. Qed.
+
+(*
+Theorem store_float64al32:
+  forall m ofs v m',
+  store Mfloat64 m ofs v = Some m' -> store Mfloat64al32 m ofs v = Some m'.
+Proof.
+  unfold store; intros.
+  destruct (valid_access_dec m Mfloat64 ofs Writable); try discriminate.
+  destruct (valid_access_dec m Mfloat64al32 ofs Writable).
+  rewrite <- H. f_equal. apply mkmem_ext; auto.
+  elim n. apply valid_access_compat with Mfloat64; auto. simpl; lia.
+Qed.
+
+Theorem storev_float64al32:
+  forall m a v m',
+  storev Mfloat64 m a v = Some m' -> storev Mfloat64al32 m a v = Some m'.
+Proof.
+  unfold storev; intros. destruct a; auto. apply store_float64al32; auto.
+Qed.
+*)
+
 (** ** Properties related to [storebytes]. *)
 
 Theorem range_perm_storebytes:
@@ -495,6 +1387,34 @@ Proof.
   econstructor; reflexivity.
   contradiction.
 Defined.
+
+(*Theorem storebytes_store:
+  forall m1 ofs chunk v vt lts m2,
+  storebytes m1 ofs (encode_val chunk (v,vt)) lts = MemorySuccess m2 ->
+  (align_chunk chunk | ofs) ->
+  store chunk m1 ofs (v,vt) lts = MemorySuccess m2.
+Proof.
+  unfold storebytes, store. intros.
+  destruct (range_perm_neg_dec m1 ofs (ofs + Z.of_nat (length (encode_val chunk (v,vt)))) Dead); inv H.
+  destruct (allowed_access_dec m1 chunk ofs).
+  f_equal.
+  elim n. constructor; auto.
+  rewrite encode_val_length in r. rewrite size_chunk_conv. auto.
+Qed.*)
+
+(*Theorem store_storebytes:
+  forall m1 ofs chunk v lts m2,
+  store chunk m1 ofs v lts = MemorySuccess m2 ->
+  storebytes m1 ofs (encode_val chunk v) lts = MemorySuccess m2.
+Proof.
+  unfold storebytes, store. intros.
+  destruct (allowed_access_dec m1 chunk ofs); inv H.
+  destruct (range_perm_neg_dec m1 ofs (ofs + Z.of_nat (length (encode_val chunk v))) Dead).
+  f_equal.
+  elim n.
+  rewrite encode_val_length. rewrite <- size_chunk_conv.
+  unfold allowed_access in *. destruct a. auto.
+Qed.*)
 
 Section STOREBYTES.
 Variable m1: mem.
@@ -535,6 +1455,52 @@ Qed.
 
 Local Hint Resolve perm_storebytes_1 perm_storebytes_2: mem.
 
+Theorem storebytes_valid_access_1:
+  forall chunk' ofs',
+    valid_access m1 chunk' ofs' -> valid_access m2 chunk' ofs'.
+Proof.
+  intros. inv H. constructor; try red; auto with mem.
+Qed.
+
+Theorem storebytes_valid_access_2:
+  forall chunk' ofs',
+  valid_access m2 chunk' ofs' -> valid_access m1 chunk' ofs'.
+Proof.
+  intros. inv H. constructor; try red; auto with mem.
+Qed.
+
+Local Hint Resolve storebytes_valid_access_1 storebytes_valid_access_2: mem.
+
+Theorem storebytes_allowed_access_1:
+  forall chunk' ofs',
+    allowed_access m1 chunk' ofs' -> allowed_access m2 chunk' ofs'.
+Admitted.
+  
+Theorem storebytes_allowed_access_2:
+  forall chunk' ofs',
+  allowed_access m2 chunk' ofs' -> allowed_access m1 chunk' ofs'.
+Admitted.
+
+Local Hint Resolve storebytes_valid_access_1 storebytes_valid_access_2: mem.
+
+Theorem storebytes_valid_block_1:
+  forall ofs, valid_addr m1 ofs -> valid_addr m2 ofs.
+Proof.
+  unfold valid_addr; intros. destruct H as [lo [hi H]]. exists lo. exists hi.
+  unfold storebytes in *. destruct (range_perm_neg_dec m1 ofs (ofs + Z.of_nat (Datatypes.length bytes)) Dead); inv STORE.
+  simpl. auto.
+Qed.
+
+Theorem storebytes_valid_block_2:
+  forall ofs, valid_addr m2 ofs -> valid_addr m1 ofs.
+Proof.
+  unfold valid_addr; intros. destruct H as [lo [hi H]]. exists lo. exists hi.
+  unfold storebytes in *. destruct (range_perm_neg_dec m1 ofs (ofs + Z.of_nat (Datatypes.length bytes)) Dead); inv STORE.
+  simpl. auto.
+Qed.
+
+Local Hint Resolve storebytes_valid_block_1 (*storebytes_valid_block_2*): mem.
+
 Theorem storebytes_range_perm:
   range_perm_neg m1 ofs (ofs + Z.of_nat (length bytes)) Dead.
 Proof.
@@ -545,6 +1511,71 @@ Proof.
   auto.
 Qed.
 
+Theorem loadbytes_storebytes_same:
+  loadbytes m2 ofs (Z.of_nat (length bytes)) = MemorySuccess bytes.
+Admitted.
+(*Proof.
+  intros. assert (STORE2:=STORE). unfold storebytes in STORE2. unfold loadbytes.
+  destruct (range_perm_neg_dec m1 ofs (ofs + Z.of_nat (length bytes)) Dead);
+  try discriminate.
+  rewrite pred_dec_true.
+  decEq. inv STORE2; simpl. rewrite PMap.gss. rewrite Nat2Z.id.
+  apply getN_setN_same.
+  red; eauto with mem.
+Admitted.*)
+
+Theorem loadbytes_storebytes_disjoint:
+  forall ofs' len,
+    len >= 0 ->
+    Intv.disjoint (ofs', ofs' + len) (ofs, ofs + Z.of_nat (length bytes)) ->
+    loadbytes m2 ofs' len = loadbytes m1 ofs' len.
+Admitted.
+(*Proof.
+  intros. unfold loadbytes.
+  destruct (range_perm_neg_dec m1 ofs' (ofs' + len) Dead);
+    destruct (range_perm_neg_dec m2 ofs' (ofs' + len) Dead).
+  rewrite storebytes_mem_contents. decEq.
+  rewrite PMap.gsspec. destruct (peq b). subst b'.
+  apply getN_setN_disjoint. rewrite Z2Nat.id by lia. intuition congruence.
+  auto.
+  admit.
+  admit.
+  red; auto with mem.
+  apply pred_dec_false.
+  red; intros; elim n. red; auto with mem.
+Qed.*)
+
+Theorem loadbytes_storebytes_other:
+  forall ofs' len,
+  len >= 0 ->
+  ofs' + len <= ofs
+  \/ ofs + Z.of_nat (length bytes) <= ofs' ->
+  loadbytes m2 ofs' len = loadbytes m1 ofs' len.
+Admitted.
+(*Proof.
+  intros. apply loadbytes_storebytes_disjoint; auto.
+  destruct H0; auto. apply Intv.disjoint_range; auto.
+Qed.*)
+
+Theorem load_storebytes_other:
+  forall chunk ofs',
+    ofs' + size_chunk chunk <= ofs
+    \/ ofs + Z.of_nat (length bytes) <= ofs' ->
+    load chunk m2 ofs' = load chunk m1 ofs'.
+Admitted.
+(*Proof.
+  intros. unfold load.
+  destruct (valid_access_dec m1 chunk ofs' Readable).
+  rewrite pred_dec_true.
+  rewrite storebytes_mem_contents. decEq.
+  rewrite PMap.gsspec. destruct (peq b). subst b'.
+  rewrite getN_setN_outside. auto. rewrite <- size_chunk_conv. intuition congruence.
+  auto.
+  destruct v; split; auto. red; auto with mem.
+  apply pred_dec_false.
+  red; intros; elim n. destruct H0. split; auto. red; auto with mem.
+Qed.
+*)
 End STOREBYTES.
 
 Lemma setN_concat:
@@ -556,8 +1587,96 @@ Proof.
   simpl length. rewrite Nat2Z.inj_succ. simpl. rewrite IHbytes1. decEq. lia.
 Qed.
 
+Theorem storebytes_concat:
+  forall m ofs bytes1 lts1 m1 bytes2 lts2 m2,
+  storebytes m ofs bytes1 lts1 = MemorySuccess m1 ->
+  storebytes m1 (ofs + Z.of_nat(length bytes1)) bytes2 lts2 = MemorySuccess m2 ->
+  storebytes m ofs (bytes1 ++ bytes2) (lts1 ++ lts2) = MemorySuccess m2.
+Admitted.
+(*Proof.
+  intros. generalize H; intro ST1. generalize H0; intro ST2.
+  unfold storebytes; unfold storebytes in ST1; unfold storebytes in ST2.
+  destruct (range_perm_neg_dec m ofs (ofs + Z.of_nat(length bytes1)) Dead); try congruence.
+  destruct (range_perm_neg_dec m1 (ofs + Z.of_nat(length bytes1)) (ofs + Z.of_nat(length bytes1) + Z.of_nat(length bytes2)) Dead); try congruence.
+  destruct (range_perm_neg_dec m ofs (ofs + Z.of_nat (length (bytes1 ++ bytes2))) Dead).
+  inv ST1; inv ST2; simpl. decEq. apply mkmem_ext; auto.
+  rewrite PMap.gss.  rewrite setN_concat. symmetry. apply PMap.set2.
+  elim n.
+  rewrite app_length. rewrite Nat2Z.inj_add. red; intros.
+  destruct (zlt ofs0 (ofs + Z.of_nat(length bytes1))).
+  apply r. lia.
+  eapply perm_storebytes_2; eauto. apply r0. lia.
+Qed.*)
+
+Theorem storebytes_split:
+  forall m ofs bytes1 bytes2 lts1 lts2 m2,
+  storebytes m ofs (bytes1 ++ bytes2) (lts1 ++ lts2) = MemorySuccess m2 ->
+  exists m1,
+     storebytes m ofs bytes1 lts1 = MemorySuccess m1
+  /\ storebytes m1 (ofs + Z.of_nat(length bytes1)) bytes2 lts2 = MemorySuccess m2.
+Proof.
+Admitted.
+     (* intros.
+  destruct (range_perm_storebytes m ofs bytes1) as [m1 ST1].
+  red; intros. exploit storebytes_range_perm; eauto. rewrite app_length.
+  rewrite Nat2Z.inj_add. lia.
+  destruct (range_perm_storebytes m1 (ofs + Z.of_nat (length bytes1)) bytes2) as [m2' ST2].
+  red; intros. eapply perm_storebytes_1; eauto. exploit storebytes_range_perm.
+  eexact H. instantiate (1 := ofs0). rewrite app_length. rewrite Nat2Z.inj_add. lia.
+  auto.
+  assert (Some m2 = Some m2').
+  rewrite <- H. eapply storebytes_concat; eauto.
+  inv H0.
+  exists m1; split; auto.
+Qed.*)
+
+Theorem store_int64_split:
+  forall m ofs v lts m',
+  store Mint64 m ofs v lts = MemorySuccess m' -> Archi.ptr64 = false ->
+  exists m1,
+     store Mint32 m ofs (if Archi.big_endian then atom_map Val.hiword v else atom_map Val.loword v) lts = MemorySuccess m1
+  /\ store Mint32 m1 (ofs + 4) (if Archi.big_endian then atom_map Val.loword v else atom_map Val.hiword v) lts = MemorySuccess m'.
+Admitted.
+(*Proof.
+  intros.
+  exploit store_allowed_access_3; eauto. intros [A B]. simpl in *.
+  exploit store_storebytes. eexact H. intros SB.
+  rewrite encode_val_int64 in Sby auto.
+  exploit storebytes_split. eexact SB. intros [m1 [SB1 SB2]].
+  rewrite encode_val_length in SB2. simpl in SB2.
+  exists m1; split.
+  apply storebytes_store. exact SB1.
+  simpl. apply Z.divide_trans with 8; auto. exists 2; auto.
+  apply storebytes_store. exact SB2.
+  simpl. apply Z.divide_add_r. apply Z.divide_trans with 8; auto. exists 2; auto. exists 1; auto.
+Qed.*)
+
 (** ** Properties related to [alloc]. *)
 
 Global Opaque Mem.store Mem.load Mem.storebytes Mem.loadbytes.
+
+(*Global Hint Resolve
+  Mem.valid_not_valid_diff
+  Mem.valid_access_valid_addr
+  Mem.valid_access_perm
+  Mem.valid_access_load
+  (*Mem.load_valid_access*)
+  Mem.loadbytes_range_perm
+  Mem.valid_access_store
+  Mem.perm_store_1
+  Mem.perm_store_2
+  Mem.store_valid_block_1
+  Mem.store_valid_block_2
+  Mem.store_valid_access_1
+  Mem.store_valid_access_2
+  (*Mem.store_valid_access_3*)
+  Mem.storebytes_range_perm
+  Mem.perm_storebytes_1
+  Mem.perm_storebytes_2
+  Mem.storebytes_valid_access_1
+  Mem.storebytes_valid_access_2
+  Mem.storebytes_valid_block_1
+  Mem.storebytes_valid_block_2
+: mem.*)
 
 End Mem.
